added tactics to take advantage of monotonic functions; sensitive to associativity and commutativity

util/meta/tactic/monotonicity.lean
@@ -1,5 +1,11 @@
 
+import data.dlist
+
 import util.logic
+import util.data.traversable
+import util.control.monad
+
+import util.data.list
 
 variables {a b c p : Prop}
 
@@ -135,6 +141,573 @@ example {α β : Type} (p : α → β → Prop) (r : α → Prop) (s : β → Pr
 begin
   introv_mono h₀ h₁,
   apply h ; assumption,
+end
+
+meta inductive mono_function (elab : bool := tt)
+ | non_assoc : expr elab → list (expr elab) → list (expr elab) → mono_function
+ | assoc : expr elab → option (expr elab) → option (expr elab) → mono_function
+ | assoc_comm : expr elab → expr elab → mono_function
+
+meta instance : decidable_eq mono_function :=
+by mk_dec_eq_instance
+
+meta def mono_function.to_tactic_format : mono_function → tactic format
+ | (mono_function.non_assoc fn xs ys) := do
+  fn' ← pp fn,
+  xs' ← mmap pp xs,
+  ys' ← mmap pp ys,
+  return format!"{fn'} {xs'} _ {ys'}"
+ | (mono_function.assoc fn xs ys) := do
+  fn' ← pp fn,
+  xs' ← pp xs,
+  ys' ← pp ys,
+  return format!"{fn'} {xs'} _ {ys'}"
+ | (mono_function.assoc_comm fn xs) := do
+  fn' ← pp fn,
+  xs' ← pp xs,
+  return format!"{fn'} _ {xs'}"
+
+meta instance : has_to_tactic_format mono_function :=
+{ to_tactic_format := mono_function.to_tactic_format }
+
+meta structure mono_ctx :=
+  (to_rel : expr → expr → expr)
+  (function : mono_function)
+  (left right rel_def : expr)
+
+meta def mono_ctx.to_tactic_format (ctx : mono_ctx) : tactic format :=
+do fn  ← pp ctx.function,
+   l   ← pp ctx.left,
+   r   ← pp ctx.right,
+   rel ← pp ctx.rel_def,
+   return format!"{{ function := {fn}\n, left  := {l}\n, right := {r}\n, rel_def := {rel} }"
+
+meta instance has_to_tactic_format_mono_ctx : has_to_tactic_format mono_ctx :=
+{ to_tactic_format := mono_ctx.to_tactic_format }
+
+-- meta instance : has_reflect mono_function :=
+-- by mk_has_reflect_instance
+
+meta def parse_imp' : list expr → expr → tactic (expr × list expr)
+ | xs e :=
+   do `(%%e₀ → %%e₁) ← return e | return (e,xs),
+      if (¬ e₁.has_var) then
+        parse_imp' (e₀ :: xs) e₁
+      else
+        return (e,xs)
+
+meta def parse_imp := parse_imp' []
+
+@[user_attribute]
+meta def monotonicity.attr : user_attribute :=
+{ name  := `monotonic
+, descr := "monotonicity of functions wrt relations: R₀ x y → R₁ (f x) (f y)" }
+
+open list has_map
+
+meta def is_mvar : expr → bool
+ | (expr.mvar _ _ _) := tt
+ | _ := ff
+
+meta def compare (unif : bool) (e₀ e₁ : expr) : tactic unit := do
+if unif then do
+guard (¬ is_mvar e₀ ∧ ¬ is_mvar e₁),
+unify e₀ e₁
+else is_def_eq e₀ e₁
+
+meta def delete_expr (unif : bool) (e : expr)
+: list expr → tactic (option (list expr))
+ | [] := return none
+ | (x :: xs) :=
+(compare unif e x >> return (some xs))
+<|>
+(map (cons x) <$> delete_expr xs)
+
+meta def match_ac' (unif : bool)
+: list expr → list expr → tactic (list expr × list expr × list expr)
+ | es (x :: xs) := do
+    es' ← delete_expr unif x es,
+    match es' with
+     | (some es') := do
+       (c,l,r) ← match_ac' es' xs, return (x::c,l,r)
+     | none := do
+       (c,l,r) ← match_ac' es xs, return (c,l,x::r)
+    end
+ | es [] := do
+return ([],es,[])
+
+meta def match_ac (unif : bool) (l : list expr) (r : list expr)
+: tactic (list expr × list expr × list expr) :=
+do (s',l',r') ← match_ac' unif l r,
+   s' ← mmap instantiate_mvars s',
+   l' ← mmap instantiate_mvars l',
+   r' ← mmap instantiate_mvars r',
+   return (s',l',r')
+
+meta def match_prefix (unif : bool)
+: list expr → list expr → tactic (list expr × list expr × list expr)
+| (x :: xs) (y :: ys) :=
+  (do compare unif x y,
+      prod.map ((::) x) id <$> match_prefix xs ys)
+<|> return ([],x :: xs,y :: ys)
+| xs ys := return ([],xs,ys)
+
+meta class elaborable (α : Type) (β : inout Type) :=
+  (elaborate : α → tactic β)
+
+export elaborable (elaborate)
+
+meta instance : elaborable pexpr expr :=
+⟨ to_expr ⟩
+
+meta instance elaborable_list {α α'} [elaborable α α'] : elaborable (list α) (list α') :=
+⟨ mmap (elaborate _) ⟩
+
+meta def mono_function.elaborate : mono_function ff → tactic mono_function
+| (mono_function.non_assoc x y z) :=
+mono_function.non_assoc <$> elaborate _ x
+                        <*> elaborate _ y
+                        <*> elaborate _ z
+| (mono_function.assoc x y z) :=
+mono_function.assoc <$> elaborate _ x
+                    <*> traverse (elaborate _) y
+                    <*> traverse (elaborate _) z
+| (mono_function.assoc_comm x y) :=
+mono_function.assoc_comm <$> elaborate _ x
+                         <*> elaborate _ y
+
+
+meta instance elaborable_mono_function : elaborable (mono_function ff) mono_function :=
+⟨ mono_function.elaborate ⟩
+
+meta instance prod_elaborable {α α' β β' : Type} [elaborable α α']  [elaborable β β']
+: elaborable (α × β) (α' × β') :=
+⟨ λ i, prod.rec_on i (λ x y, prod.mk <$> elaborate _ x <*> elaborate _ y) ⟩
+
+run_cmd
+do xs ← mmap to_expr [``(1),``(2),``(3)],
+   ys ← mmap to_expr [``(1),``(2),``(4)],
+   x ← match_prefix ff xs ys,
+   p ← elaborate _ ([``(1),``(2)] , [``(3)], [``(4)]),
+   guard $ x = p
+
+/--
+`(prefix,left,right,suffix) ← match_assoc unif l r` finds the
+longest prefix and suffix common to `l` and `r` and
+returns them along with the differences  -/
+meta def match_assoc (unif : bool) (l : list expr) (r : list expr)
+: tactic (list expr × list expr × list expr × list expr) :=
+do (pre,l₁,r₁) ← match_prefix unif l r,
+   (suf,l₂,r₂) ← match_prefix unif (reverse l₁) (reverse r₁),
+   return (pre,reverse l₂,reverse r₂,reverse suf)
+
+run_cmd
+do xs ← mmap to_expr [``(1),``(2),``(3),``(6),``(7)],
+   ys ← mmap to_expr [``(1),``(2),``(4),``(5),``(6),``(7)],
+   x ← match_assoc ff xs ys,
+   p ← elaborate _ ([``(1), ``(2)], [``(3)], ([``(4), ``(5)], [``(6), ``(7)])),
+   guard (x = p)
+
+meta def check_ac : expr → tactic (bool × bool × option (expr × expr) × expr)
+ | (expr.app (expr.app f x) y) :=
+   do t ← infer_type x,
+      a ← try_core $ to_expr ``(is_associative %%t %%f) >>= mk_instance,
+      c ← try_core $ to_expr ``(is_commutative %%t %%f) >>= mk_instance,
+      i ← try_core (do
+          v ← mk_meta_var t,
+          prod.mk <$> (to_expr ``(is_left_id %%t %%f %%v) >>= mk_instance)
+                  <*> instantiate_mvars v),
+      return (a.is_some,c.is_some,i,f)
+ | _ := return (ff,ff,none,expr.var 1)
+
+run_cmd
+do x ← to_expr ``(7 + 3 : ℕ) >>= check_ac,
+   x ← pp x.2.2.1,
+   guard $ x.to_string = "(some (add_monoid_to_is_left_id, 0))"
+
+open dlist has_map
+
+meta def parse_assoc_chain' (f : expr) : expr → tactic (dlist expr)
+ | e :=
+ (do (expr.app (expr.app f' x) y) ← return e,
+     is_def_eq f f',
+     (++) <$> parse_assoc_chain' x <*> parse_assoc_chain' y)
+<|> return (singleton e)
+
+meta def parse_assoc_chain (f : expr) : expr → tactic (list expr) :=
+map dlist.to_list ∘ parse_assoc_chain' f
+
+open monad (mmap₂')
+
+meta def find_one_difference (unif : bool)
+: list expr → list expr → tactic (list expr × expr × expr × list expr)
+ | (x :: xs) (y :: ys) :=
+   do c ← try_core (compare unif x y),
+      if c.is_some
+      then prod.map (cons x) id <$> find_one_difference xs ys
+      else do
+        guard (xs.length = ys.length),
+        mmap₂' (compare unif) xs ys,
+        return ([],x,y,xs)
+ | _ _ := failed
+
+meta def fold_assoc (op : expr) : option (expr × expr) → list expr → option expr
+| _ (x::xs) := some $ foldl (expr.app ∘ expr.app op) x xs
+| none []   := none
+| (some (inst,x₀)) [] := some x₀
+
+meta def fold_assoc1 (op : expr) : list expr → option expr
+| (x::xs) := some $ foldl (expr.app ∘ expr.app op) x xs
+| []   := none
+
+meta def same_function_aux
+: list expr → list expr → expr → expr → tactic (expr × list expr × list expr)
+ | xs₀ xs₁ (expr.app f₀ a₀) (expr.app f₁ a₁) :=
+   same_function_aux (a₀ :: xs₀) (a₁ :: xs₁) f₀ f₁
+ | xs₀ xs₁ e₀ e₁ := is_def_eq e₀ e₁ >> return (e₀,xs₀,xs₁)
+
+meta def same_function : expr → expr → tactic (expr × list expr × list expr) :=
+same_function_aux [] []
+
+meta def parse_mono_function (l r : expr)
+: tactic (expr × expr × mono_function) :=
+do (full_f,ls,rs) ← same_function l r,
+   (a,c,i,f) ← check_ac l,
+   if a
+   then if c
+   then do
+     (s,ls,rs) ← monad.join (match_ac ff
+                   <$> parse_assoc_chain f l
+                   <*> parse_assoc_chain f r),
+     l' ← fold_assoc f i ls,
+     r' ← fold_assoc f i rs,
+     s' ← fold_assoc1 f s,
+     return (l',r',mono_function.assoc_comm f s')
+   else do -- a ∧ ¬ c
+     (pre,ls,rs,suff) ← monad.join (match_assoc ff
+                   <$> parse_assoc_chain f l
+                   <*> parse_assoc_chain f r),
+     l'   ← fold_assoc f i ls,
+     r'   ← fold_assoc f i rs,
+     let pre'  := fold_assoc1 f pre,
+     let suff' := fold_assoc1 f suff,
+     return (l',r',mono_function.assoc f pre' suff')
+   else do -- ¬ a
+     (xs₀,x₀,x₁,xs₁) ← find_one_difference ff ls rs,
+     return (x₀,x₁,mono_function.non_assoc full_f xs₀ xs₁)
+
+meta def parse_mono_function' (l r : pexpr) :=
+do l' ← to_expr l,
+   r' ← to_expr r,
+   parse_mono_function l' r'
+
+run_cmd
+do parse_mono_function' ``(1 + 3 + 2 + 6) ``(4 + 2 + 1 + 5) >>= trace,
+   parse_mono_function' ``([1] ++ [3] ++ [2] ++ [6]) ``([4] ++ [2] ++ ([1] ++ [5]))
+     >>= trace,
+   parse_mono_function' ``([1] ++ [3] ++ [2] ++ [2]) ``([1] ++ [5] ++ ([4] ++ [2]))
+     >>= trace
+
+meta def monotonicity_goal : expr → tactic (expr × expr × mono_ctx)
+ | `(%%e₀ → %%e₁) :=
+  do (l,r,f) ← parse_mono_function e₀ e₁,
+     t₀ ← infer_type e₀,
+     t₁ ← infer_type e₁,
+     rel_def ← to_expr ``(λ x₀ x₁, (x₀ : %%t₀) → (x₁ : %%t₁)),
+     return (e₀, e₁,
+            { function := f
+            , left := l, right := r
+            , to_rel := expr.pi `x binder_info.default
+            , rel_def := rel_def })
+ | (expr.app (expr.app rel e₀) e₁) :=
+  do (l,r,f) ← parse_mono_function e₀ e₁,
+     return (e₀, e₁,
+            { function := f
+            , left := l, right := r
+            , to_rel := expr.app ∘ expr.app rel
+            , rel_def := rel })
+ | _ := fail "invalid monotonicity goal"
+
+private meta def match_head (p : expr) : expr → expr → tactic expr
+ | e t :=
+(unify t p >> instantiate_mvars e)
+<|>
+do (expr.pi _ _ d b) ← return t | failed,
+   v ← mk_meta_var d,
+   match_head (expr.app e v) (b.instantiate_var v)
+
+meta def bin_op_left (f : expr)  : option expr → expr → expr
+| none e := e
+| (some e₀) e₁ := f.mk_app [e₀,e₁]
+
+meta def bin_op (f a b : expr) : expr :=
+f.mk_app [a,b]
+
+meta def bin_op_right (f : expr) : expr → option expr → expr
+| e none := e
+| e₀ (some e₁) := f.mk_app [e₀,e₁]
+
+meta def mk_fun_app : mono_function → expr → expr
+ | (mono_function.non_assoc f x y) z := f.mk_app (x ++ z :: y)
+ | (mono_function.assoc f x y) z := bin_op_left f x (bin_op_right f z y)
+ | (mono_function.assoc_comm f x) z := f.mk_app [z,x]
+
+meta inductive mono_law
+ | assoc : expr × expr → expr × expr → mono_law
+ | other : expr → mono_law
+
+meta def mono_law.to_tactic_format : mono_law → tactic format
+ | (mono_law.other e) := do e ← pp e, return format!"other {e}"
+ | (mono_law.assoc (x₀,x₁) (y₀,y₁)) :=
+do x₀ ← pp x₀,
+   x₁ ← pp x₁,
+   y₀ ← pp y₀,
+   y₁ ← pp y₁,
+   return format!"assoc {x₀}; {x₁} | {y₀}; {y₁}"
+
+meta instance has_to_tactic_format_mono_law : has_to_tactic_format mono_law :=
+{ to_tactic_format := mono_law.to_tactic_format }
+
+meta def mk_rel (ctx : mono_ctx) (f : expr → expr) : expr :=
+ctx.to_rel (f ctx.left) (f ctx.right)
+
+meta def mk_pattern (ctx : mono_ctx) : option mono_law :=
+match ctx.function with
+ | (mono_function.assoc f (some x) (some y)) :=
+   mono_law.assoc
+       ( mk_rel ctx (λ i, bin_op f x (bin_op f i y))
+       , mk_rel ctx (λ i, bin_op f i y))
+       ( mk_rel ctx (λ i, bin_op f (bin_op f x i) y)
+       , mk_rel ctx (λ i, bin_op f x i))
+ | (mono_function.assoc f (some x) none) :=
+   mono_law.other $
+   ctx.to_rel (mk_fun_app ctx.function ctx.left)
+              (mk_fun_app ctx.function ctx.right)
+ | (mono_function.assoc f none (some y)) :=
+   mono_law.other $
+   ctx.to_rel (mk_fun_app ctx.function ctx.left)
+              (mk_fun_app ctx.function ctx.right)
+ | (mono_function.assoc f none none) :=
+   none
+ | _ :=
+   mono_law.other $
+   ctx.to_rel (mk_fun_app ctx.function ctx.left)
+              (mk_fun_app ctx.function ctx.right)
+end
+
+-- meta def mk_associative_pattern : option expr → option expr → expr := _
+
+meta def match_rule (pat : expr) (r : name) : tactic expr :=
+do  r' ← mk_const r,
+    t  ← infer_type r',
+    match_head pat r' t
+
+meta def find_lemma (pat : expr) : list name → tactic expr
+ | [] := failed
+ | (r :: rs) :=
+ do match_rule pat r <|> find_lemma rs
+
+meta def match_chaining_rules (ls : list name) (x₀ x₁ : expr) : tactic expr :=
+do x' ← to_expr ``(%%x₁ → %%x₀),
+   r₀ ← find_lemma x' ls,
+   r₁ ← find_lemma x₁ ls,
+   return (expr.app r₀ r₁)
+
+meta def find_rule (ls : list name) : mono_law → tactic (expr)
+ | (mono_law.assoc (x₀,x₁) (y₀,y₁)) :=
+(match_chaining_rules ls x₀ x₁)
+<|> (match_chaining_rules ls y₀ y₁)
+ | (mono_law.other p) := find_lemma p ls
+
+meta def list_meta_vars (e : expr) : list expr :=
+e.fold [] (λ e' _ es, if is_mvar e' then e' :: es else es)
+
+universes u v
+
+lemma apply_rel {α : Sort u} (R : α → α → Sort v) {x y : α}
+  (x' y' : α)
+  (h : R x y)
+  (hx : x = x')
+  (hy : y = y')
+: R x' y' :=
+by { rw [← hx,← hy], apply h }
+
+meta def monotonicity1 : tactic unit :=
+do (l,r,g) ← target >>= instantiate_mvars >>= monotonicity_goal,
+   ns ← attribute.get_instances `monotonic,
+   p ← mk_pattern g,
+   rule ← find_rule ns p,
+   x ← to_expr ``(apply_rel %%(g.rel_def) %%l %%r %%rule),
+   tactic.apply x,
+   solve1 (refl <|> ac_refl <|> `[simp only [is_associative.assoc]]),
+   solve1 (refl <|> ac_refl <|> `[simp only [is_associative.assoc]])
+
+@[monotonic]
+lemma add_mono {α : Type} {x y z : α} [ordered_semiring α]
+  (h : x ≤ y)
+: x + z ≤ y + z :=
+add_le_add_right h _
+
+@[monotonic]
+lemma sub_mono_left {α : Type} {x y z : α} [ordered_comm_group α]
+  (h : x ≤ y)
+: x - z ≤ y - z :=
+sub_le_sub_right h _
+
+@[monotonic]
+lemma sub_mono_right {α : Type} {x y z : α} [ordered_comm_group α]
+  (h : y ≤ x)
+: z - x ≤ z - y :=
+sub_le_sub_left h _
+
+lemma bar
+  (h : 3 + 6 ≤ 4 + 5)
+: 1 + 3 + 2 + 6 ≤ 4 + 2 + 1 + 5 :=
+begin
+  monotonicity1,
+  apply h
+end
+
+lemma bar'
+  (h : 3 ≤ (4 : ℤ))
+  (h' : 5 ≤ (6 : ℤ))
+: (1 + 3 + 2) - 6 ≤ (4 + 2 + 1 : ℤ) - 5 :=
+begin
+  transitivity (1 + 3 + 2 - 5 : ℤ),
+  monotonicity1,
+  apply h',
+  monotonicity1,
+  monotonicity1,
+  apply h
+end
+
+@[simp]
+def list.le {α : Type*} [has_le α] : list α → list α → Prop
+ | (x::xs) (y::ys) := x ≤ y ∧ list.le xs ys
+ | [] [] := true
+ | _ _ := false
+
+@[simp]
+instance {α : Type*} [has_le α] : has_le (list α) :=
+⟨ list.le ⟩
+
+@[refl]
+lemma list.le_refl {α : Type*} [preorder α] {xs : list α}
+: xs ≤ xs :=
+begin
+  induction xs with x xs,
+  { trivial },
+  { simp [has_le.le,list.le],
+    split, apply le_refl, apply ih_1 }
+end
+
+@[trans]
+lemma list.le_trans {α : Type*} [preorder α]
+  {xs zs : list α} (ys : list α)
+  (h  : xs ≤ ys)
+  (h' : ys ≤ zs)
+: xs ≤ zs :=
+begin
+  revert ys zs,
+  induction xs with x xs
+  ; intros ys zs h h'
+  ; cases ys with y ys
+  ; cases zs with z zs
+  ; try { cases h ; cases h' ; done },
+  { refl },
+  { simp [has_le.le,list.le],
+    split,
+    apply le_trans h.left h'.left,
+    apply ih_1 _ h.right h'.right, }
+end
+
+@[monotonic]
+lemma list_le_mono_left {α : Type*} [preorder α] {xs ys zs : list α}
+  (h : xs ≤ ys)
+: xs ++ zs ≤ ys ++ zs :=
+begin
+  revert ys,
+  induction xs with x xs ; intros ys h,
+  { cases ys, refl, cases h },
+  { cases ys with y ys, cases h, simp [has_le.le,list.le] at *,
+    revert h, apply and.imp_right,
+    apply ih_1 }
+end
+
+@[monotonic]
+lemma list_le_mono_right {α : Type*} [preorder α] {xs ys zs : list α}
+  (h : xs ≤ ys)
+: zs ++ xs ≤ zs ++ ys :=
+begin
+  revert ys zs,
+  induction xs with x xs ; intros ys zs h,
+  { cases ys, { simp }, cases h  },
+  { cases ys with y ys, cases h, simp [has_le.le,list.le] at *,
+    rw [list.append_cons _ x,list.append_cons _ y],
+    apply list.le_trans (zs ++ [y] ++ xs),
+    { apply list_le_mono_left,
+      induction zs with z zs,
+      { simp [has_le.le,list.le], apply h.left },
+      { simp [has_le.le,list.le], split, apply le_refl,
+        apply ih_1_1, } },
+    { apply ih_1 h.right, } }
+end
+
+lemma bar_bar'
+  (h : [] ++ [3] ++ [2] ≤ [1] ++ [5] ++ [4])
+: [] ++ [3] ++ [2] ++ [2] ≤ [1] ++ [5] ++ ([4] ++ [2]) :=
+begin
+  monotonicity1,
+  apply h
+end
+
+lemma bar_bar''
+  (h : [3] ++ [2] ++ [2] ≤ [5] ++ [4] ++ [])
+: [1] ++ ([3] ++ [2]) ++ [2] ≤ [1] ++ [5] ++ ([4] ++ []) :=
+begin
+  monotonicity1,
+  apply h,
+end
+
+lemma bar_bar
+  (h : [3] ++ [2] ≤ [5] ++ [4])
+: [1] ++ [3] ++ [2] ++ [2] ≤ [1] ++ [5] ++ ([4] ++ [2]) :=
+begin
+  monotonicity1,
+  apply h
+end
+
+def P (x : ℕ) := 7 ≤ x
+def Q (x : ℕ) := x ≤ 7
+
+@[monotonic]
+lemma P_mono {x y : ℕ}
+  (h : x ≤ y)
+: P x → P y :=
+by { intro h', apply le_trans h' h }
+
+@[monotonic]
+lemma Q_mono {x y : ℕ}
+  (h : y ≤ x)
+: Q x → Q y :=
+by apply le_trans h
+
+example (x y z : ℕ)
+  (h : x ≤ y)
+: P (x + z) → P (z + y) :=
+begin
+  monotonicity1,
+  monotonicity1,
+  apply h,
+end
+
+example (x y z : ℕ)
+  (h : y ≤ x)
+: Q (x + z) → Q (z + y) :=
+begin
+  monotonicity1,
+  monotonicity1,
+  apply h,
 end
 
 end tactic.interactive
