util/algebra/group.lean
@@ -1,0 +1,16 @@
+
+instance monoid_to_is_left_id {α : Type*} [monoid α]
+: is_left_id α (*) 1 :=
+⟨ monoid.one_mul ⟩
+
+instance monoid_to_is_right_id {α : Type*} [monoid α]
+: is_right_id α (*) 1 :=
+⟨ monoid.mul_one ⟩
+
+instance add_monoid_to_is_left_id {α : Type*} [add_monoid α]
+: is_left_id α (+) 0 :=
+⟨ add_monoid.zero_add ⟩
+
+instance add_monoid_to_is_right_id {α : Type*} [add_monoid α]
+: is_right_id α (+) 0 :=
+⟨ add_monoid.add_zero ⟩
