util/control/monad.lean
@@ -18,4 +18,14 @@ lemma bind_map (f : α → β) (x : m α) (g : β → m γ)
 : f <$> x >>= g = x >>= g ∘ f :=
 sorry
 
+def mmap₂  (f : α → β → m γ) : list α → list β → m (list γ)
+| (x :: xs) (y :: ys) := (::) <$> f x y <*> mmap₂ xs ys
+| [] _ := pure []
+| _ [] := pure []
+
+def mmap₂'  (f : α → β → m γ) : list α → list β → m punit
+| (x :: xs) (y :: ys) := f x y *> mmap₂' xs ys
+| [] _ := pure punit.star
+| _ [] := pure punit.star
+
 end monad
